##### 夹逼定理
- 夹逼定理
	- [[函数极限]]夹逼定理
		- 如果 $g(x)\leq f(x)\leq h(x)$, 且 $\displaystyle\lim_{x\rightarrow a}g(x)=\displaystyle\lim_{x\rightarrow a}h(x)=A$
		- 则 $\displaystyle\lim_{x\rightarrow a}f(x)=A$
	- [[数列极限]]夹逼定理
		- 如果 $y_n\leq a_n\leq z_n$, 且$\displaystyle\lim^{}_{n\to \infty}y_n=\lim^{}_{n\to \infty}z_n=L$ 
		- 则 $\displaystyle\lim^{}_{n\to\infty}a_n=L$

>[!example]- 夹逼定理
>- 证明$\displaystyle \lim_{n\to\infty}\sqrt{1+\frac{1}{n}}=1$
>	- 因为 $\displaystyle1<\sqrt{1+\frac{1}{n}}<1+\frac{1}{n}$, 且 $\displaystyle\lim_{n\to\infty}1=1$ , $\displaystyle\lim_{n\to\infty}(1+\frac{1}{n})=1$ , 所以成立
>- 证明 $\displaystyle \lim_{n\to\infty}a_n=\lim_{n\to\infty}\frac{\sin(n)}{n^2}=0$ 
>	- 因为 $\displaystyle -\frac{1}{n^2}\leq\frac{\sin(n)}{n^2}\leq\frac{1}{n^2}$, 且 $\displaystyle\lim_{n\to\infty}-\frac{1}{n^2}=0$ , $\displaystyle\lim_{n\to\infty}\frac{1}{n^2}=0$ , 所以成立



